w64x4/proof/Fp_w64x4_proof_mulm.ec
@@ -67,18 +67,18 @@ wp; skip; smt(Array16.get_setE Array16.set_set_if).
 qed.
 
 
-equiv muln_spec:
+equiv muln_spec aa bb:
  M.bn_muln ~ ASpecFp.muln:
-  ImplZZ a{1} a{2} /\ ImplZZ b{1} b{2}
+  ImplZZ a{1} a{2} /\ ImplZZ b{1} b{2} /\ aa = a{1} /\ bb = b{1}
   ==> 
   ImplZZ2 res{1}.`4 res{2}
-     /\ res{1}.`1 = W64.zero /\ !res{1}.`2 /\ !res{1}.`3.
+     /\ res{1}.`1 = W64.zero /\ !res{1}.`2 /\ !res{1}.`3 /\ valR2 res{1}.`4 = valR aa * valR bb.
 proof.
 transitivity 
  MulOps.mulR
- ( ={a,b} ==> res{1}.`2=res{2}.`1 /\ res{1}.`3=res{2}.`2 /\ res{1}.`4=res{2}.`3 /\  res{1}.`1 = W64.zero )
- ( ImplZZ a{1} a{2} /\ ImplZZ b{1} b{2} 
-   ==> !res{1}.`1 /\ !res{1}.`2 /\ ImplZZ2 res{1}.`3 res{2}).
+ ( ={a,b} ==> res{1}.`2=res{2}.`1 /\ res{1}.`3=res{2}.`2 /\ res{1}.`4=res{2}.`3 /\  res{1}.`1 = W64.zero  )
+ ( ImplZZ a{1} a{2} /\ ImplZZ b{1} b{2} /\ aa = a{1} /\ bb = b{1}
+   ==> !res{1}.`1 /\ !res{1}.`2 /\ ImplZZ2 res{1}.`3 res{2} /\ valR2 res{1}.`3 = valR aa * valR bb).
 + by move=> /> &1 &2 H1 H2; exists (a{1},b{1}).
 + by move=> /> /#.
 + proc; simplify.
@@ -86,13 +86,13 @@ transitivity
           1 <= k{2} <= nlimbs ).
   wp. call mul1acc_eq. wp. skip. smt.
    (* by wp; call mul1acc_eq; wp; skip => /> /#. *)
-  by wp; call mul1first_eq; wp; skip => /> /#.
+  wp; call mul1first_eq; wp; skip => /> .
 + proc.
   transitivity {1}
     { (_of,_cf,r) <@ MulOps.mulR(a,b); }
     ( ={a,b} ==> ={_cf,_of,r} )
-    ( ImplZZ a{1} a{2} /\ ImplZZ b{1} b{2} ==> !_cf{1} /\ !_of{1} /\ ImplZZ2 r{1} r{2} ).
-  + by move=> /> &1; exists a{1} b{1}; auto.
+    ( ImplZZ a{1} a{2} /\ ImplZZ b{1} b{2} /\ aa = a{1} /\ bb = b{1} ==> !_cf{1} /\ !_of{1} /\ ImplZZ2 r{1} r{2} /\ valR2 r{1} = valR aa * valR bb ).
+  progress. exists a{1} b{1}; auto.
   + by move=> /> *.
   + by inline MulOps.mulR; sim.
   + by ecall {1} (mulR_ph a{1} b{1}); wp; skip.
@@ -195,16 +195,50 @@ apply Array8.ext_eq. progress. smt.
 qed.
 
 
-lemma dbn_set0_correct :
-  phoare[ M.bn_set0 : true  ==> W64x4.valR res = 0 ] = 1%r.
-proc.
-while (i <= nlimbs 
-  /\ (forall j, 0 <= j < i => a.[j]%Array4 = W64.zero)) (nlimbs - i). progress.
-wp.  skip.  progress. smt().  smt(@Array4). smt(). wp.  skip. progress. smt(). smt().
-rewrite - zeroRE. congr.
-apply Array4.ext_eq. progress.  rewrite H1. smt(). 
-rewrite /zeroR. smt(@Array4).
+(* lemma dbn_set0_correct : *)
+(*   phoare[ M.bn_set0 : true  ==> W64x4.valR res = 0 ] = 1%r. *)
+(* proc. *)
+(* while (i <= nlimbs  *)
+(*   /\ (forall j, 0 <= j < i => a.[j]%Array4 = W64.zero)) (nlimbs - i). progress. *)
+(* wp.  skip.  progress. smt().  smt(@Array4). smt(). wp.  skip. progress. smt(). smt(). *)
+(* rewrite - zeroRE. congr. *)
+(* apply Array4.ext_eq. progress.  rewrite H1. smt().  *)
+(* rewrite /zeroR. smt(@Array4). *)
+(* qed. *)
+
+
+
+
+op oneR : R = (of_list W64.zero [W64.one; W64.zero; W64.zero; W64.zero])%Array4.
+
+lemma oneRE: ImplZZ oneR 1.
+rewrite /oneR /valR /bnk.
+have ->: range 0 4 = [0;1;2;3].  rewrite range_ltn. auto.
+rewrite range_ltn. auto. rewrite range_ltn. auto.
+simplify. rewrite range_ltn. auto.
+simplify. rewrite range_geq. auto. auto.
+rewrite big_consT.
+rewrite big_consT.
+rewrite big_consT.
+rewrite big_consT.
+rewrite big_nil.
+simplify. smt(@Int).
 qed.
+
+
+lemma bn_set1_correct :
+  phoare[ M.bn_set1 : true  ==> W64x4.valR res = 1 ] = 1%r.
+proc.
+while (0 < i <= nlimbs 
+  /\ (forall j, 1 <= j < i => a.[j]%Array4 = W64.zero) /\ a.[0]%Array4 = W64.one) (nlimbs - i). progress.
+wp.  skip.  progress. smt(). smt().  smt(@Array4). smt(@Array4). smt(). wp.  skip. progress. smt(@Array4). smt().
+rewrite - oneRE. congr.
+apply Array4.ext_eq. progress.  
+case (x = 0). progress. progress.
+rewrite H2. smt(). 
+rewrite /oneR. smt(@Array4).
+qed.
+
 
 
 lemma dbn_copy_correct x :
@@ -216,6 +250,18 @@ while (a = x /\ i <= dnlimbs
 wp.  skip.  progress. smt. smt. smt. wp.  skip. progress. smt. smt.
 apply Array8.ext_eq. progress. smt. 
 qed.
+
+
+lemma bn_copy_correct x :
+  phoare[ M.bn_copy :  arg = x  ==> res = x ] = 1%r.
+proc.
+while (a = x /\ i <= nlimbs 
+  /\ (forall j, 0 <= j < i => r.[j]%Array4 = x.[j]%Array4)
+  ) (dnlimbs - i). progress.
+wp.  skip.  progress. smt. smt. smt. wp.  skip. progress. smt. smt.
+apply Array4.ext_eq. progress. smt. 
+qed.
+
 
 
 equiv dcminusP_spec:
@@ -331,7 +377,7 @@ lemma bn_expand_correct : forall a,
        have gen : forall n, 0 <= n => foldr (fun (w : W64.t) (r0 : int) => to_uint w + W64x8.M * r0) 0
                      (nseq n  W64.zero) = 0.
        apply intind. progress. rewrite nseq0. simplify. auto.
-       progress. rewrite nseqS. auto. search  foldr. simplify. rewrite H2. auto.
+       progress. rewrite nseqS. auto. simplify. rewrite H2. auto.
        apply gen. auto.
     rewrite W64x4.R.bn2seq. rewrite /bn_seq. rewrite /to_list. 
     pose f := (fun (w : W64.t) (r0 : int) => to_uint w + W64x8.M * r0).
@@ -377,7 +423,7 @@ ecall {1} (bn_shrink_correct xrf{1}). wp. skip. progress. smt.
 seq 1 1 : (valR a{1} = a{2} /\ valR r{1} = r{2} /\ ImplZZ p{1} P /\ k{2} = 64 * nlimbs
     /\ W64x8.valR2 xr{1} = xr{2} /\ valR xrfd{1} = xrf{2} 
     /\  W64x8.valR xrfn{1} = xrfn{2}).
-call muln_spec. skip. progress.
+ecall  (muln_spec xrfd{1} p{1}). skip. progress.
 seq 1 1 : (valR a{1} = a{2} /\ valR r{1} = r{2} /\ ImplZZ p{1} P /\ k{2} = 64 * nlimbs
     /\ W64x8.valR2 xr{1} = xr{2} /\ W64x4.valR xrfd{1} = xrf{2} 
     /\ W64x8.valR xrfn{1} = xrfn{2}
@@ -412,7 +458,7 @@ equiv bnreduce_spec:
  M.bn_breduce ~ ASpecFp.redm:
   valR a{1} = a{2}
   /\ ImplZZ p{1} P
-  /\ valR r{1} = (nlimbs ^ (64 * nlimbs) %/ P) 
+  /\ valR r{1} = (4 ^ (64 * nlimbs) %/ P) 
   /\ 0 < P < W64x4.modulusR
   /\ 0 <= a{2} < P * P
   /\ 0 < P < 2 ^ (64 * nlimbs)
@@ -459,3 +505,507 @@ qed.
 
 
 
+lemma q (a b p : int) : 0 <= a < p => 0 <= b < p => a * b < p * p.
+smt. qed.
+
+equiv mulm_cspec:
+ M.mulm ~ CSpecFp.mulm:
+  valR a{1} = a{2}
+  /\ valR b{1} = b{2}
+  /\ valR a{1} < P
+  /\ valR b{1} < P
+  /\ ImplZZ p{1} P
+  /\ valR r{1} = (4 ^ (64 * nlimbs) %/ P) 
+  (* /\ 0 < P < 2 ^ (64 * nlimbs) *)
+   ==> valR res{1} =  res{2} .
+proc. 
+call bnreduce_spec.
+ecall (muln_spec a{1} b{1}).
+wp. skip. progress.  smt. smt.
+smt. rewrite H6.  
+apply q. smt.
+smt. smt. smt.
+smt.
+qed.
+
+
+equiv mulm_spec:
+ M.mulm ~ ASpecFp.mulm:
+  valR a{1} = asint a{2}
+  /\ valR b{1} = asint b{2}
+  /\ valR p{1} = P
+  /\ valR r{1} = (4 ^ (64 * nlimbs) %/ P) 
+   ==> valR res{1} = asint res{2} .
+transitivity CSpecFp.mulm
+ (valR a{1} = a{2}
+  /\ valR b{1} = b{2}
+  /\ valR a{1} < P
+  /\ valR b{1} < P
+  /\ ImplZZ p{1} P
+  /\ valR r{1} = (4 ^ (64 * nlimbs) %/ P) 
+   ==> valR res{1} =  res{2})
+ (a{1} = asint a{2} /\ b{1} = asint b{2}  ==> res{1} = asint res{2}).
+move=> /> &1 &2 H1 H2 H3 H4; exists (valR a{1}, valR b{1}). smt. progress.
+conseq mulm_cspec. 
+conseq mulm_eq.
+qed.
+
+
+
+
+require import BitEncoding.
+import BS2Int.
+
+require Abstract_exp_proof_8.
+
+
+
+clone import Abstract_exp_proof_8 as Exp with type R  <- t,
+                                                 op P <- P,
+                                                 op Rsize <- 256,
+                                                 op valR <- W64x4.valR,
+                                                 op of_int <- bn_ofint,
+                                                 op idR <- bn_ofint 1,
+                                                 op ( ** ) <- Int.( * ),
+                                                 op ( *** ) <=  fun a b => bn_ofint ((valR%W64x4 a * valR%W64x4 b) %% P)
+proof*.
+realize Rsize_max. smt(). qed.
+realize Rsize_pos. smt(). qed.
+realize valr_pos. smt (@W64x4). qed.
+realize iii.  rewrite /Rbits. 
+progress. rewrite  size_int2bs. auto. qed.
+realize valr_ofint.  progress.
+rewrite bn_ofintK. smt.
+qed.
+realize P_pos. smt. qed.
+realize ofint_valr. smt(@W64x4). qed.
+realize rbits_bitsr. 
+progress. rewrite /Rbits. rewrite /bitsR. 
+  have ->: (valR (bn_ofint (bs2int x)))%W64x4 = bs2int x.
+rewrite bn_ofintK. smt. smt. qed.
+realize bitsr_rbits. 
+rewrite /Rbits. rewrite /bitsR.
+progress.
+rewrite int2bsK. auto. simplify. progress. smt(bnk_cmp).
+have : 0 <= valR  x < W64x4.M ^ nlimbs.
+rewrite /valR. 
+apply (bnk_cmp nlimbs).
+progress. smt.
+smt(@W64x4).
+qed.
+realize exp_prop7. progress. smt. qed.
+realize exp_prop6. progress.
+have ->: (valR (bn_ofint ((valR a * valR b) %% P)) * valR c) %% P
+  = ((valR a * valR ((bn_ofint ((valR b * valR c) %% P)))) %% P). 
+rewrite valr_ofint. smt.
+rewrite valr_ofint. smt.
+rewrite modzMml.
+rewrite modzMmr. smt.
+auto.
+qed.
+realize exp_prop5. progress. 
+rewrite valr_ofint. progress. smt. simplify. 
+rewrite modz_small. smt.
+smt. qed.
+realize mult_valr. progress. smt. qed.
+realize idR_leP. smt. qed.
+
+
+
+  
+op R : W64.t Array8.t.
+axiom R_prop : valR R = 4 ^ (64 * nlimbs) %/ P.
+
+module MultM = {
+  proc ith_bit = M.ith_bit
+  proc swapr   = M.swapr
+  proc opr (p:W64.t Array4.t, a:W64.t Array4.t,
+             b:W64.t Array4.t) : W64.t Array4.t = {
+    var r;
+    r <@ M.mulm(R,p,a,b);
+    return r;
+  }
+}.
+
+
+
+lemma ones64 : (2^64  - 1)  = 18446744073709551615. smt(). qed.
+lemma swap_lemma :
+      equiv[ MultM.swapr ~ Spec.swapr :
+              a{2} = x{1} /\ b{2} = y{1} /\ swap_0{1} = as_w64 c{2} ==> ={res}].
+proc.  simplify.
+seq 2 0 : (i{1} = 0 /\ a{2} = x{1} /\ b{2} = y{1} /\ swap_0{1} = as_w64 c{2} /\ 
+   ((as_bool swap_0{1} => mask{1} = (of_int 18446744073709551615)%W64 )
+              /\ (as_bool swap_0{1} = false => mask{1} = (of_int 0)%W64))).
+wp. skip. progress. smt(@W64). smt.
+while {1} (0 <= i{1} /\ ((as_bool swap_0{1} => mask{1} = (of_int 18446744073709551615)%W64 )
+              /\ (as_bool swap_0{1} = false => mask{1} = (of_int 0)%W64)) 
+   /\ (forall j, 0 <= j < i{1} => (x{1}.[j])%Array4 = (if as_bool swap_0{1} then (b{2}.[j]) else (a{2}.[j]))%Array4 )  
+   /\ (forall j, 0 <= j < i{1} => (y{1}.[j])%Array4 = (if as_bool swap_0{1} then (a{2}.[j]) else (b{2}.[j]))%Array4 )  
+   /\ (forall j, i{1} <= j => (x{1}.[j])%Array4 =  (a{2}.[j]))%Array4
+   /\ (forall j, i{1} <= j => (y{1}.[j])%Array4 =  (b{2}.[j]))%Array4
+ ) (nlimbs - i{1} + 1).
+progress. wp.  skip.  progress.   smt().
+case (j <  i{hr}). progress.  timeout 15. smt.
+progress.
+have : j = i{hr}. smt.
+progress.
+have ->: (x{hr}.[i{hr} <-
+    x{hr}.[i{hr}] `^` (x{hr}.[i{hr}] `^` y{hr}.[i{hr}] `&` mask{hr})].[i{hr}])%Array4
+ = (x{hr}.[i{hr}] `^` (x{hr}.[i{hr}] `^` y{hr}.[i{hr}] `&` mask{hr}))%Array4. smt.
+case (as_bool swap_0{hr}). progress.
+rewrite H4. auto.  rewrite H0. auto. rewrite H5. auto. rewrite - ones64. 
+have -> : ((a{m}.[i{hr}])%Array4 `^` (b{m}.[i{hr}])%Array4 `&`
+ (of_int W64.max_uint)%W64) = a{m}.[i{hr}]%Array4 `^` ((b{m}.[i{hr}])%Array4 `&`
+ (of_int W64.max_uint)%W64). smt. 
+have ->: ((b{m}.[i{hr}])%Array4 `&` (of_int W64.max_uint)%W64) = ((b{m}.[i{hr}])%Array4). smt.
+smt(@W64).
+progress. rewrite H4. auto.  rewrite H1. smt(). auto. 
+case (j <  i{hr}). progress.  timeout 15. smt.
+progress.
+have : j = i{hr}. smt.
+progress.
+have ->: (y{hr}.[i{hr} <-
+   y{hr}.[i{hr}] `^` (x{hr}.[i{hr}] `^` y{hr}.[i{hr}] `&` mask{hr})].[i{hr}])%Array4
+ = (y{hr}.[i{hr}] `^` (x{hr}.[i{hr}] `^` y{hr}.[i{hr}] `&` mask{hr}))%Array4. smt.
+case (as_bool swap_0{hr}). progress.
+rewrite H4. auto.  rewrite H0. auto. rewrite H5. auto. rewrite - ones64. 
+have -> : ((a{m}.[i{hr}])%Array4 `^` (b{m}.[i{hr}])%Array4 `&`
+ (of_int W64.max_uint)%W64) = a{m}.[i{hr}]%Array4 `^` ((b{m}.[i{hr}])%Array4 `&`
+ (of_int W64.max_uint)%W64). smt. 
+have ->: ((b{m}.[i{hr}])%Array4 `&` (of_int W64.max_uint)%W64) = ((b{m}.[i{hr}])%Array4). smt.
+smt(@W64).
+progress. rewrite H4. auto.  rewrite H1. smt(). smt(@W64).
+smt. smt. smt.
+skip. progress. smt().   smt().   smt(). 
+case (c{2} = false). progress.  
+apply Array4.ext_eq.  progress. rewrite H5. progress. smt(). rewrite /as_bool. rewrite /as_w64. simplify. smt(@W64).
+apply Array4.ext_eq.  progress. rewrite H6. progress. smt(). rewrite /as_bool. rewrite /as_w64. simplify. smt(@W64).
+progress. have ->: c{2} = true. smt(). simplify.
+progress. 
+apply Array4.ext_eq.  progress. rewrite H5. progress. smt(). rewrite /as_bool. rewrite /as_w64. simplify. smt(@W64).
+apply Array4.ext_eq.  progress. rewrite H6. progress. smt(). rewrite /as_bool. rewrite /as_w64. simplify. smt(@W64).
+qed.
+
+
+
+
+lemma okll : 
+  equiv[ MultM.opr ~ M.mulm :
+            a{1} = a{2} /\ b{1} = b{2} /\  p{1} = p{2} /\ r{2} = R ==>
+            ={res}].
+proc. inline M.mulm. sim. wp.  skip.  auto.
+qed.
+
+lemma okl : 
+  equiv[ MultM.opr ~ Exp.Spec.mul :
+            a{1} = a{2} /\ b{1} = b{2} /\  valR p{1} = P /\ valR a{1} < P /\ valR b{1} < P ==>
+            ={res} /\ valR res{1} < P].
+symmetry.
+transitivity ASpecFp.mulm 
+  (ImplFp arg{1}.`1  arg{2}.`1 /\ ImplFp arg{1}.`2  arg{2}.`2 ==> ImplFp res{1} res{2} )
+  (ImplFp a{2} a{1} /\ ImplFp b{2} b{1} /\  valR p{2} = P /\ valR a{2} < P /\ valR b{2} < P ==>
+            ImplFp res{2} res{1} /\ valR res{2} < P).
+    progress. 
+  exists (inzp (valR a{1}), inzp (valR b{1}) )%W64x4. progress.
+rewrite inzpK. rewrite modz_small. smt. smt.
+rewrite inzpK. rewrite modz_small. smt. smt.
+rewrite inzpK. rewrite modz_small. smt. smt.
+rewrite inzpK. rewrite modz_small. smt. smt.
+progress. smt. 
+proc.  wp. skip.  progress.
+       rewrite H H0.
+smt.
+auto.
+symmetry. 
+transitivity M.mulm 
+  (={p,a,b} /\ r{2} = R ==> ={res})
+  (ImplFp a{1} a{2} /\
+  ImplFp b{1} b{2} /\ ImplZZ p{1} P /\ valR a{1} < P /\ valR b{1} < P /\ r{1} = R ==> ImplFp res{1} res{2} /\ valR res{1} < P).
+progress. exists (R,p{1},a{1},b{1}). progress. auto.
+conseq okll. auto.
+conseq mulm_spec. progress. rewrite H4. apply R_prop. 
+progress.  smt.
+qed.
+
+module MM = {
+  proc ith_bit (kk:W64.t Array4.t, ctr:W64.t) : W64.t = {
+    var bit:W64.t;
+    var c1:W64.t;
+    var c2:W64.t;
+    var r:W64.t;
+    
+    c1 <- (ctr `>>` (W8.of_int 6));
+    c2 <- (ctr - (c1 * (W64.of_int 64)));
+    r <- kk.[(W64.to_uint c1)]%Array4;
+    bit <@ IB.ith_bit64 (r, c2);
+    return (bit);
+  }
+
+}.
+lemma ith_bit_lemmaEq :
+      equiv[ MM.ith_bit ~ M.ith_bit : ={arg} ==> ={res}].
+proc.
+seq 2 4 : (={c1, c2,kk}). wp.
+skip. progress.
+have -> : 63 = 2^6 - 1. smt().
+rewrite and_mod. auto. simplify.
+have x:  to_uint (ctr{2} `>>` (of_int 6)%W8) = to_uint ctr{2} %/ 64. smt.
+rewrite to_uint_eq.
+auto.
+rewrite to_uintB.  rewrite /(\ule). smt.
+rewrite to_uintM_small.  smt.
+rewrite  shr_div_le.
+auto. simplify. smt.
+sim.
+qed.
+
+
+
+
+lemma ith_bit_lemma' :
+      equiv[ M.ith_bit ~ Spec.ith_bit : arg{1}.`1 = arg{2}.`1 /\  W64.to_uint arg{1}.`2 = arg{2}.`2 /\
+ 0 <= ctr{2} && ctr{2} < 256 ==>
+              ={res} /\ (res{2} = W64.one \/ res{2} = W64.zero)].
+transitivity MM.ith_bit
+   (={arg} ==> ={res})
+   (arg{1}.`1 = arg{2}.`1 /\  W64.to_uint arg{1}.`2 = arg{2}.`2 /\
+ 0 <= ctr{2} && ctr{2} < 256 ==>
+              ={res} /\ (res{2} = W64.one \/ res{2} = W64.zero)).
+progress. smt(). smt().
+symmetry. conseq ith_bit_lemmaEq. auto. auto.
+proc.
+seq 3 0 : (to_uint c1{1} = (to_uint ctr{1} %/ 64) /\ to_uint c2{1} = (to_uint ctr{1} %% 64) /\ to_uint ctr{1} = ctr{2}
+  /\ r{1} = kk{1}.[(to_uint ctr{1} %/ 64)]%Array4 /\ r{2} = kk{1} /\ 0 <= ctr{2} && ctr{2} < 256 ).
+wp.  skip. progress.
+smt.
+rewrite modzE.
+have <-: to_uint (ctr{1} `>>` (of_int 6)%W8) = to_uint ctr{1} %/ 64. smt.
+rewrite to_uintB. rewrite /(\ule). smt.
+smt.
+smt.
+exists* r{1}, c2{1}. elim*. progress.
+call {1} (ithbit64 r_L c2_L). skip.
+progress. smt. smt.
+rewrite /ith_bitword64.  rewrite H0.
+rewrite /ith_bitR. rewrite /Rbits. rewrite /valR.
+rewrite /ith_bit.
+rewrite /as_word.
+rewrite /as_w64.
+have ->: (kk{1}.[to_uint ctr{1} %/ 64])%Array4.[to_uint ctr{1} %% 64]
+  = nth false (int2bs 256 ((valR kk{1}))%W64x4) (to_uint ctr{1}) .
+rewrite - get_w2bits.
+rewrite - get_to_list.
+have -> : (W64.w2bits (nth witness ((to_list kk{1}))%Array4 (to_uint ctr{1} %/ 64)))
+ = ((nth witness (map W64.w2bits (to_list kk{1}))%Array4 (to_uint ctr{1} %/ 64))).
+rewrite - (nth_map witness witness W64.w2bits). progress.   smt. smt.
+auto.
+have -> : (nth witness (map W64.w2bits ((to_list kk{1}))%Array4)
+     (to_uint ctr{1} %/ 64))
+ = (nth [] (map W64.w2bits ((to_list kk{1}))%Array4)
+     (to_uint ctr{1} %/ 64)).
+rewrite (nth_change_dfl [] witness). progress.  smt. smt. auto.
+rewrite - (BitChunking.nth_flatten false 64 (map W64.w2bits ((to_list kk{1}))%Array4) (to_uint ctr{1})).
+rewrite  List.allP. progress. timeout 5.
+have : exists z, z \in ((to_list kk{1}))%Array4 /\ x = W64.w2bits z.
+apply mapP. auto. elim. progress.
+have ->: (flatten (map W64.w2bits ((to_list kk{1}))%Array4))  = (int2bs 256 ((valR kk{1}))%W64x4).
+have -> : (valR kk{1})%W64x4 = bs2int (flatten (map W64.w2bits ((to_list kk{1}))%Array4)).
+rewrite /bnk.
+have ->: range 0 4 = [0;1;2;3].  rewrite range_ltn. auto.
+rewrite range_ltn. auto. rewrite range_ltn. auto.
+simplify. rewrite range_ltn. auto.
+simplify. rewrite range_geq. auto. auto.
+rewrite big_consT.
+rewrite big_consT.
+rewrite big_consT.
+rewrite big_consT.
+rewrite big_nil.
+rewrite /to_list.
+have ->: 4 = 0 + 1 + 1 + 1 + 1 . smt().
+rewrite   mkseqS. auto.
+rewrite   mkseqS. auto.
+rewrite   mkseqS. auto.
+rewrite   mkseqS. auto.
+rewrite mkseq0. simplify.
+rewrite flatten_cons.
+rewrite flatten_cons.
+rewrite flatten_cons.
+rewrite flatten_cons.
+rewrite flatten_nil.
+rewrite cats0.
+rewrite bs2int_cat.
+rewrite bs2int_cat.
+rewrite bs2int_cat. simplify.
+smt.
+have ->: 256 = size (flatten (map W64.w2bits ((to_list kk{1}))%Array4)).
+rewrite /to_list.
+have ->: 4 = 0 + 1 + 1 + 1 + 1 . smt().
+rewrite   mkseqS. auto.
+rewrite   mkseqS. auto.
+rewrite   mkseqS. auto.
+rewrite   mkseqS. auto.
+rewrite mkseq0. simplify.
+rewrite flatten_cons.
+rewrite flatten_cons.
+rewrite flatten_cons.
+rewrite flatten_cons.
+rewrite flatten_nil.
+rewrite size_cat.
+rewrite size_cat.
+rewrite size_cat.
+rewrite size_cat.
+simplify. auto.
+rewrite  bs2intK. auto. auto.
+auto. smt().
+qed.
+
+
+lemma expm_real_spec : 
+      equiv[ Exp.M1.iterop_spec ~ Exp.M7(MultM).iterop :
+            ImplZZ m{2} P /\
+            ={x} /\
+            bs2int n{1} = valR n{2} /\ size n{1} = 256 /\ valR x{1} < P ==>
+            ={res}].
+apply (Exp.iterop_real_speac MultM _ _ _). 
+transitivity M.swapr
+  (={arg} ==> ={res})
+  (a{2} = x{1} /\ b{2} = y{1} /\ swap_0{1} = (as_w64 c{2}) ==>
+          ={res}).
+progress. smt(). smt().
+proc. sim.
+symmetry.
+transitivity Spec.swapr
+  (={arg} ==> ={res})
+  (a{1} = x{2} /\ b{1} = y{2} /\ swap_0{2} = (as_w64 c{1}) ==>
+          ={res}).
+smt(). smt().
+proc. sim.
+symmetry. conseq swap_lemma. smt(). 
+transitivity MultM.ith_bit
+  (={arg} ==> ={res})
+  (arg{1}.`1 = arg{2}.`1 /\ ImplWord ctr{1} ctr{2} /\ 0 <= ctr{2} && ctr{2} < 256 ==>
+          ={res} /\ (res{2} = W64.one \/ res{2} = W64.zero)).
+smt(). smt().
+proc. sim.
+conseq ith_bit_lemma'.
+conseq okl. smt(). auto. auto.
+qed.
+
+lemma to_uintP: forall (x y : R), valR (x *** y) = (valR x * valR y) %% P.
+progress. rewrite /( *** ). smt.
+qed.
+
+
+lemma kk :  forall (n : int), 0 <= n => forall (a : zp) (b : t), valR%W64x4 b < P =>
+  ImplFp b a =>
+  ImplFp ((^) b n) (inzp (asint a ^ n)).
+apply intind. progress.
+rewrite exp_prop1.
+have -> : (asint a ^ 0) = 1. smt.
+rewrite /asint.
+have -> : (Sub.val (inzp 1))%Sub = 1. smt.
+smt.
+progress.
+have ->: ((^) b (i + 1)) = b *** ((^) b  i).
+rewrite exp_prop3. auto. auto.  auto.
+rewrite exp_prop2.
+rewrite exp_prop7. smt.
+have ->: inzp (asint a ^ (i + 1)) =  inzp (asint a * (asint a ^ i)).
+smt.
+have ->:  inzp (asint a * (asint a ^ i)) = (inzp (asint a)) * (inzp (asint a ^ i)).
+smt.
+rewrite - H2. 
+have ->: asint (inzp (valR%W64x4 b) * inzp (valR%W64x4 b ^ i))
+  = (asint (inzp (valR%W64x4 b)) * (asint  (inzp (valR%W64x4 b ^ i)))) %% P.
+smt.
+have ih :  ImplFp (b ^ i)  (inzp (valR%W64x4 b ^ i)).
+smt.
+rewrite - ih.
+have ->: asint (inzp (valR%W64x4 b)) = valR%W64x4 b. smt.
+simplify. 
+rewrite  to_uintP /=. done.
+qed.
+
+
+lemma left_end :
+ equiv[ ASpecFp.expm ~ Exp.M1.iterop_spec  :
+    ImplFp x{2} a{1} /\  bs2int n{2}  = valR b{1} /\ valR%W64x4 x{2} < P ==> ImplFp res{2} res{1}]. 
+proc.
+wp.  skip.  progress.
+rewrite  (kk (bs2int n{2}) _ a{1}). smt. auto. auto. smt.
+qed.
+
+
+lemma right_end : 
+ equiv[ M7(MultM).iterop ~ M.expm : r{2} = R /\ ={m,x,n} ==> ={res} ].
+proc. sim.
+seq  7  13 : (={x1,x2,x3,x4,d,ctr,n,m} /\ r{2} = R).
+call (_:true). sim.
+call (_:true). sim.
+wp. 
+    call okll.
+ecall {2} (bn_copy_correct x{2}).
+wp. 
+call (_:true). sim. 
+call {2} bn_set1_correct.
+call {2} bn_set1_correct. wp. skip. progress.
+smt. smt.
+while (={x1,x2,x3,x4,d,ctr,n,m} /\ r{2} = R). wp.
+call (_:true). sim. wp.
+call (_:true). sim. wp.
+call okll.
+call okll.
+call (_:true). sim. wp.
+call (_:true). sim. wp. 
+call (_:true). sim. wp. 
+skip. progress.
+smt.
+skip.
+progress. 
+qed.
+
+
+lemma expm_correct : 
+      equiv[ ASpecFp.expm ~ M.expm :
+             ImplZZ m{2} P /\
+             asint a{1} = valR x{2} /\
+             b{1} = n{2}  /\ 
+             valR x{2} < P /\ 
+             r{2} = R
+             ==> asint res{1} = valR{2}%W64x4 res{2}]. 
+simplify.
+transitivity Exp.M1.iterop_spec
+  (ImplFp x{2} a{1} /\  bs2int n{2} = valR b{1} /\ size n{2} = 256  /\ valR%W64x4 x{2} < P ==> ImplFp res{2} res{1})
+  (ImplZZ m{2} P /\
+             x{1} =  x{2} /\
+            bs2int n{1} = valR n{2} /\ size n{1} = 256 /\ valR x{2} < P /\ r{2} = R ==>
+            res{1} =  res{2}).
+progress.
+exists (x{2}, int2bs 256 (valR b{1})).
+progress. smt.
+smt.
+smt.
+smt.
+smt. smt.
+conseq left_end.  smt.
+symmetry.
+transitivity M7(MultM).iterop
+ (r{1} = R /\ ={m,x,n}  ==> ={res})
+ (p{2} = P /\ size n{2} = 256 /\
+             x{1} =  x{2} /\
+                         ImplZZ m{1} P /\
+             valR n{1} = bs2int  n{2}  /\ valR x{2} < P  ==>
+            res{1} =  res{2}).
+progress.
+exists (m{1}, x{1}, n{1}). progress. smt(). smt.
+smt(). auto.
+symmetry.
+conseq right_end. smt().
+progress.
+symmetry.
+conseq expm_real_spec. progress.
+smt().
+smt.
+progress.
+qed.
